iris/SpecFiledup.v
@@ -42,6 +42,7 @@ Require Import SpecPanic.
 Require Import IntrDefs.
 Require Import CpuOwn.
 From Kernel Require KernelSyms.
+Require Import InodeRef.
 Local Open Scope Z_scope.
 
 
@@ -71,7 +72,7 @@ Local Open Scope Z_scope.
 
 (* ------------------------------------------------------------------ *)
 
-Definition wp_filedup_sconf_body `{!riscvGS Σ, !lockG Σ, !sieG Σ, !fileG Σ, !fdslotG Σ} `{GEN : GenId} `{CID : CpuId} (γl γf : gname)
+Definition wp_filedup_sconf_body `{!riscvGS Σ, !lockG Σ, !sieG Σ, !fileG Σ, !fdslotG Σ, !irefNameG Σ} `{GEN : GenId} `{CID : CpuId} (γl γf : gname)
     (k : nat) (q : Qp) (Cf : fcontent)
     (m : regfile) (n : nat) (eb : bool) (p : mword 64) (C : iProp Σ) (K : nat) (b : bool) :=
   let pcE : mword 64 := mword_of_int KernelSyms.filedup in
@@ -105,7 +106,7 @@ Definition wp_filedup_sconf_body `{!riscvGS Σ, !lockG Σ, !sieG Σ, !fileG Σ, 
 
 Module Type FILEDUP.
   Parameter wp_filedup_sconf :
-    forall `{!riscvGS Σ, !lockG Σ, !sieG Σ, !fileG Σ, !fdslotG Σ} `{GEN : GenId} `{CID : CpuId} (γl γf : gname)
+    forall `{!riscvGS Σ, !lockG Σ, !sieG Σ, !fileG Σ, !fdslotG Σ, !irefNameG Σ} `{GEN : GenId} `{CID : CpuId} (γl γf : gname)
       (k : nat) (q : Qp) (Cf : fcontent)
       (m : regfile) (n : nat) (eb : bool) (p : mword 64) (C : iProp Σ) (K : nat) (b : bool),
       wp_filedup_sconf_body γl γf k q Cf m n eb p C K b.
